Protocols/Synapse.lean
@@ -3,19 +3,23 @@
 --
 
 import Batteries
+import Aesop
 
 abbrev State := Nat × Nat × Nat
 
+@[aesop unsafe [cases]]
 inductive Reachable : State -> Prop where
   | start {i} : Reachable (i, 0, 0)
   | t1 {i d v} : Reachable (i + 1, d, v) -> Reachable (i + d, 0, v + 1)
   | t2 {i d v} : Reachable (i, d, v + 1) -> Reachable (i + d + v, 1, 0)
   | t3 {i d v} : Reachable (i + 1, d, v) -> Reachable (i + d + v, 1, 0)
 
+@[aesop unsafe [cases]]
 inductive Unsafe : State -> Prop where
   | u1 {i d v} : Unsafe (i, d + 1, v + 1)
   | u2 {i d v} : Unsafe (i, d + 2, v)
 
+@[aesop unsafe [constructors, cases]]
 inductive Config : State -> Prop where
   | c1 {i} : Config (i, 0 + 1, 0)
   | c2 {i v} : Config (i, 0, v)
@@ -29,14 +33,15 @@ open Reachable Unsafe Config
 -- Any reachable state is covered by a configuration
 
 theorem  inclusion {s : State} (r : Reachable s) : Config s := by
-  cases r with
-  | start | t1 _ => exact c2
-  | t2 _ | t3 _ => exact c1
+  -- cases r <;> constructor
+  aesop
+
 
 -- Any state, that is covered by a configuration, is not unsafe.
 
 theorem  safety {s : State} (c : Config s) (u : Unsafe s) : False := by
-  cases c <;> cases u
+  -- cases c <;> cases u
+  aesop
 
 -- Any reachable state is not unsafe.
 
@@ -48,4 +53,5 @@ theorem  valid : {s : State} -> Reachable s -> Unsafe s -> False :=
 --
 
 theorem valid' {s : State} (r : Reachable s) (u : Unsafe s) : False := by
-  cases r <;> cases u
+  -- cases r <;> cases u
+  aesop
